lib/prims.fst
@@ -17,23 +17,23 @@ module Prims
 
 kind Unop  = Type => Type           (* simple kind abbreviation *)
 kind Binop = Type => Type => Type   
-type l_not : Unop  (* prefix unary '~' *)
-type l_and : Binop (* infix binary '/\' *)
-type l_or  : Binop (* infix binary '\/' *)
-type l_iff : Binop (* infix binary '<==>' *)
-type l_imp : Binop (* infix binary '==>' *)
-type Forall : #'a:Type => ('a => Type) => Type 
-type Exists : #'a:Type => ('a => Type) => Type 
-type ForallTyp : (Type => Type) => Type (* Handled specially by the type-checker to support quantification over types of arbitrary kinds *)
-type ExistsTyp : (Type => Type) => Type (* Handled specially by the type-checker to support quantification over types of arbitrary kinds *)
-type True : Type
-type False : Type
-type EqTyp : Type => Type => Type                    (* infix binary '==' *)
-type Eq2 : #'a:Type => #'b:Type => 'a => 'b => Type  (* infix binary '==' *)
-type TypeOf : #'a:Type => 'a => Type
-type KindOf : Type => Type
-type XOR ('P:Type) ('Q:Type) = ('P \/ 'Q) /\ ~('P /\ 'Q)
-type ITE ('P:Type) ('Q:Type) ('R:Type) = ('P ==> 'Q) /\ (~'P ==> 'R) (* if/then/else in concrete syntax at the level of types/formulae *)
+
+(* Primitive logical connectives *)
+logic type l_not : Unop  (* prefix unary '~' *)
+logic type l_and : Binop (* infix binary '/\' *)
+logic type l_or  : Binop (* infix binary '\/' *)
+logic type l_iff : Binop (* infix binary '<==>' *)
+logic type l_imp : Binop (* infix binary '==>' *)
+logic type Forall : #'a:Type => ('a => Type) => Type 
+logic type Exists : #'a:Type => ('a => Type) => Type 
+logic type ForallTyp : (Type => Type) => Type (* Handled specially to support quantification over types of arbitrary kinds *)
+logic type ExistsTyp : (Type => Type) => Type (* Handled specially to support quantification over types of arbitrary kinds *)
+logic type True : Type
+logic type False : Type
+logic type EqTyp : Type => Type => Type                    (* infix binary '==' *)
+logic type Eq2 : #'a:Type => #'b:Type => 'a => 'b => Type  (* infix binary '==' *)
+logic type XOR ('P:Type) ('Q:Type) = ('P \/ 'Q) /\ ~('P /\ 'Q)
+logic type ITE ('P:Type) ('Q:Type) ('R:Type) = ('P ==> 'Q) /\ (~'P ==> 'R) (* written if/then/else in concrete syntax *)
 
 monad_lattice { (* The definition of the PURE effect is fixed; no user should ever change this *)
   PURE::
@@ -63,50 +63,46 @@ monad_lattice { (* The definition of the PURE effect is fixed; no user should ev
              and Tot ('a:Type) =
                  PURE 'a (fun 'p => (forall (x:'a). 'p x)) (fun 'p => (forall (x:'a). 'p x))
 }
-(* type assert_pure ('a:Type) ('P:Type) : PURE.WP 'a = fun ('post:PURE.Post 'a) => 'P /\ ('P ==> (forall (x:'a). 'post x)) *)
-(* type assume_pure ('a:Type) ('P:Type) : PURE.WP 'a = fun ('post:PURE.Post 'a) => 'P ==> (forall (x:'a). 'post x) *)
-
-type bool
-type b2t (b:bool) = b==true
-type unit
-assume Unit_id: forall (x:unit). x==()
-type int
-type char
-type byte
-type uint16
-type int32 = int
-type int64
-type float
+assume type bool
+assume type unit
+assume type int
+assume type char
+assume type byte
+assume type uint16
+assume type int64
+assume type float
+assume type string
+assume type array : Type => Type
+assume type ref : Type => Type
+assume type LBL : string => Type => Type
+assume type bytes
+assume type exn
+assume type HashMultiMap : Type => Type => Type
 type double = float
-type string
-type array : Type => Type
-type ref : Type => Type
-type LBL : string => Type => Type
-type bytes
-type exn
-type HashMultiMap : Type => Type => Type
+type int32 = int
+logic type b2t (b:bool) = b==true
 
-logic data type option 'a =
+type option 'a =
   | None : option 'a
   | Some : v:'a -> option 'a
 
-type heap
-logic val SelHeap : #'a:Type -> heap -> ref 'a -> 'a
-logic val UpdHeap : #'a:Type -> heap -> ref 'a -> 'a -> heap
-logic val EmpHeap : heap
-logic val InHeap  : #'a:Type -> heap -> ref 'a -> bool
+assume type heap
+assume logic val SelHeap : #'a:Type -> heap -> ref 'a -> 'a
+assume logic val UpdHeap : #'a:Type -> heap -> ref 'a -> 'a -> heap
+assume logic val EmpHeap : heap
+assume logic val InHeap  : #'a:Type -> heap -> ref 'a -> bool
 assume SelUpd1: forall ('a:Type) (h:heap) (x:ref 'a) (v:'a).{:pattern (SelHeap (UpdHeap h x v) x)} SelHeap (UpdHeap h x v) x == x
 assume SelUpd2: forall ('a:Type) ('b:Type) (h:heap) (x:ref 'a) (y:ref 'b) (v:'b).{:pattern (SelHeap (UpdHeap h y v) x)} y=!=x ==> SelHeap (UpdHeap h y v) x == SelHeap h x
 assume InHeap1:  forall ('a:Type) (h:heap) (x:ref 'a) (v:'a).{:pattern (InHeap (UpdHeap h x v) x)} InHeap (UpdHeap h x v) x == true
 assume InHeap2:  forall ('a:Type) ('b:Type) (h:heap) (x:ref 'a) (y:ref 'b) (v:'b).{:pattern (InHeap (UpdHeap h y v) x)} y=!=x ==> InHeap (UpdHeap h y v) x == InHeap h x
 
-type refset
-logic val EmptySet : refset
-logic val Singleton : ref 'a -> refset
-logic val Union : refset -> refset -> refset
-logic val Intersection : refset -> refset -> refset
-type InSet : #'a:Type => ref 'a => refset => Type
-type SetEqual : refset => refset => Type
+assume type refset
+assume logic val EmptySet : refset
+assume logic val Singleton : ref 'a -> refset
+assume logic val Union : refset -> refset -> refset
+assume logic val Intersection : refset -> refset -> refset
+logic type InSet : #'a:Type => ref 'a => refset => Type
+logic type SetEqual : refset => refset => Type
 assume InEmptySet:     forall 'a (a:ref 'a). ~(InSet a EmptySet)
 assume InSingleton:    forall 'a (a:ref 'a). InSet a (Singleton a)
 assume InSingletonInv: forall 'a 'b (a:ref 'a) (b:ref 'b). InSet a (Singleton b) <==> a==b
@@ -120,37 +116,19 @@ assume InterIdemL:     forall s1 s2. Intersection (Intersection s1 s2) s2 == Int
 assume InterdemR:      forall s1 s2. Intersection s1 (Intersection s1 s2) == Intersection s1 s2
 assume SetEqualDef:    forall s1 s2. SetEqual s1 s2 <==> (forall 'a (a:ref 'a). InSet a s1 <==> InSet a s2)
 assume SeqEqualExt:    forall s1 s2. SetEqual s1 s2 ==> s1==s2
-logic data type refs =
+type refs =
   | AllRefs : refs
   | SomeRefs : v:refset -> refs
 
-(* let zoo = function  *)
-(*   | AllRefs -> AllRefs *)
-(*   | SomeRefs v -> SomeRefs v *)
-assume val modifies : r:refs -> PURE.Tot (x:refs{x==r})
-(* let modifies (r:refs) = r *)
-(* let f1 x = *)
-(*   let r = modifies x in *)
-(*   AllRefs *)
-
-(* let foo (b:bool) = if b then 0 else 1 *)
-(* let bar a b = a *)
-
-type Modifies (mods:refs) (h:heap) (h':heap) =
+logic type Modifies (mods:refs) (h:heap) (h':heap) =
     (if b2t (is_AllRefs mods)
      then True
      else forall 'b (x:ref 'b). (b2t (InHeap h x) /\ ~(InSet x (SomeRefs.v mods))) ==> (b2t (InHeap h' x) /\ SelHeap h x==SelHeap h' x))
 
-logic data type result : Type => Type =
+type result : Type => Type =
   | V : 'a:Type -> v:'a -> result 'a
   | E : 'a:Type -> e:exn -> result 'a
   | Err : 'a:Type -> msg:string -> result 'a
-
-assume val retype : result 'a -> PURE.Tot (result 'b)
-(* let retype r = match r with *)
-(*   | V _ -> Err "impos" *)
-(*   | Err m -> Err m *)
-(*   | E e -> E e *)
 
 monad_lattice {
   STATE::
@@ -264,52 +242,52 @@ type Tuple3 'a 'b 'c =
            -> _3:'c0
           -> Tuple3 'a 'b 'c
 
-(* type Tuple4 'a 'b 'c 'd = *)
-(*   | MkTuple4: _1:'a *)
-(*            -> _2:'b *)
-(*            -> _3:'c *)
-(*            -> _4:'d *)
-(*            -> Tuple4 'a 'b 'c 'd *)
+type Tuple4 'a 'b 'c 'd =
+  | MkTuple4: _1:'a
+           -> _2:'b
+           -> _3:'c
+           -> _4:'d
+           -> Tuple4 'a 'b 'c 'd
 
-(* type Tuple5 'a 'b 'c 'd 'e = *)
-(*   | MkTuple5: _1:'a *)
-(*            -> _2:'b *)
-(*            -> _3:'c *)
-(*            -> _4:'d *)
-(*            -> _5:'e *)
-(*            -> Tuple5 'a 'b 'c 'd 'e *)
+type Tuple5 'a 'b 'c 'd 'e =
+  | MkTuple5: _1:'a
+           -> _2:'b
+           -> _3:'c
+           -> _4:'d
+           -> _5:'e
+           -> Tuple5 'a 'b 'c 'd 'e
 
-(* type Tuple6 'a 'b 'c 'd 'e 'f = *)
-(*   | MkTuple6: _1:'a *)
-(*            -> _2:'b *)
-(*            -> _3:'c *)
-(*            -> _4:'d *)
-(*            -> _5:'e *)
-(*            -> _6:'f *)
-(*            -> Tuple6 'a 'b 'c 'd 'e 'f *)
-
-
-(* type Tuple7 'a 'b 'c 'd 'e 'f 'g = *)
-(*   | MkTuple7: _1:'a *)
-(*            -> _2:'b *)
-(*            -> _3:'c *)
-(*            -> _4:'d *)
-(*            -> _5:'e *)
-(*            -> _6:'f *)
-(*            -> _7:'g *)
-(*            -> Tuple7 'a 'b 'c 'd 'e 'f 'g *)
+type Tuple6 'a 'b 'c 'd 'e 'f =
+  | MkTuple6: _1:'a
+           -> _2:'b
+           -> _3:'c
+           -> _4:'d
+           -> _5:'e
+           -> _6:'f
+           -> Tuple6 'a 'b 'c 'd 'e 'f
 
 
-(* type Tuple8 'a 'b 'c 'd 'e 'f 'g 'h = *)
-(*   | MkTuple8: _1:'a *)
-(*            -> _2:'b *)
-(*            -> _3:'c *)
-(*            -> _4:'d *)
-(*            -> _5:'e *)
-(*            -> _6:'f *)
-(*            -> _7:'g *)
-(*            -> _8:'h *)
-(*            -> Tuple8 'a 'b 'c 'd 'e 'f 'g 'h *)
+type Tuple7 'a 'b 'c 'd 'e 'f 'g =
+  | MkTuple7: _1:'a
+           -> _2:'b
+           -> _3:'c
+           -> _4:'d
+           -> _5:'e
+           -> _6:'f
+           -> _7:'g
+           -> Tuple7 'a 'b 'c 'd 'e 'f 'g
+
+
+type Tuple8 'a 'b 'c 'd 'e 'f 'g 'h =
+  | MkTuple8: _1:'a
+           -> _2:'b
+           -> _3:'c
+           -> _4:'d
+           -> _5:'e
+           -> _6:'f
+           -> _7:'g
+           -> _8:'h
+           -> Tuple8 'a 'b 'c 'd 'e 'f 'g 'h
 
 type DTuple2: 'a:Type
           => 'b:('a => Type)
@@ -347,7 +325,7 @@ type DTuple2: 'a:Type
 (*            -> _4:'d _1 _2 _3 *)
 (*            -> DTuple4 'a 'b 'c 'd *)
 
-(* logic data type Tuple5: 'a:Type *)
+(*  type Tuple5: 'a:Type *)
 (*           => 'b:('a => Type) *)
 (*           => 'c:(x:'a => 'b x => Type) *)
 (*           => 'd:(x:'a => y:'b x => z:'c x y => Type) *)
@@ -365,7 +343,7 @@ type DTuple2: 'a:Type
 (*            -> _5:'e _1 _2 _3 _4 *)
 (*            -> Tuple5 'a 'b 'c 'd 'e *)
 
-(* logic data type Tuple6: 'a:Type *)
+(*  type Tuple6: 'a:Type *)
 (*           => 'b:('a => Type) *)
 (*           => 'c:(x:'a => 'b x => Type) *)
 (*           => 'd:(x:'a => y:'b x => z:'c x y => Type) *)
@@ -386,7 +364,7 @@ type DTuple2: 'a:Type
 (*            -> _6:'f _1 _2 _3 _4 _5 *)
 (*            -> Tuple6 'a 'b 'c 'd 'e 'f *)
 
-(* logic data type Tuple7: 'a:Type *)
+(*  type Tuple7: 'a:Type *)
 (*           => 'b:('a => Type) *)
 (*           => 'c:(x:'a => 'b x => Type) *)
 (*           => 'd:(x:'a => y:'b x => z:'c x y => Type) *)
@@ -410,7 +388,7 @@ type DTuple2: 'a:Type
 (*            -> _7:'g _1 _2 _3 _4 _5 _6 *)
 (*            -> Tuple7 'a 'b 'c 'd 'e 'f 'g *)
 
-(* logic data type Tuple8: 'a:Type *)
+(*  type Tuple8: 'a:Type *)
 (*           => 'b:('a => Type) *)
 (*           => 'c:(a:'a => 'b a => Type) *)
 (*           => 'd:(a:'a => b:'b a => c:'c a b => Type) *)
@@ -441,20 +419,19 @@ type DTuple2: 'a:Type
    What about for function types? *)
 assume val op_Equality : 'a:Type -> 'b:Type -> 'a -> 'b -> PURE.Tot bool
 assume val op_disEquality : 'a:Type -> 'b:Type -> 'a -> 'b -> PURE.Tot bool
-logic type IfThenElse : 'P:Type => (u:unit{'P} => Type) => (u:unit{~'P} => Type) => Type
 
-type LT : int => int => Type
-type GT : int => int => Type
-type LTE : int => int => Type
-type GTE : int => int => Type
+logic type LT : int => int => Type    (* infix < in concrete syntax *)
+logic type GT : int => int => Type    (* infix > in concrete syntax *)
+logic type LTE : int => int => Type   (* infix <= in concrete syntax *)
+logic type GTE : int => int => Type   (* infix >= in concrete syntax *)
 type nat = i:int{i >= 0}
 type pos = n:nat{n > 0}
 
-logic data type either 'a 'b =
+type either 'a 'b =
   | Inl : v:'a -> either 'a 'b
   | Inr : v:'b -> either 'a 'b
 
-logic data type list 'cc =
+type list 'cc =
   | Nil : list 'cc
   | Cons : hd:'cc -> tl:list 'cc -> list 'cc
 
@@ -462,20 +439,16 @@ assume val fst : ('a * 'b) -> PURE.Tot 'a
 assume val snd : ('a * 'b) -> PURE.Tot 'b
 assume val Assume: 'P:Type -> unit -> (y:unit{'P})
 (* assume val Assert : 'P:Type -> x:unit{'P} -> y:unit{'P} *)
-assume val Assert : 'P:Type -> unit -> PURE.Pure unit 'P (fun (x:unit) => 'P)
+assume val Assert : 'P:Type -> unit -> PURE.Pure unit 'P (fun (x:unit) => True)
 assume val lemma : 'P:Type -> x:unit{'P} -> z:unit{'P}
 assume val unreachable : x:unit{LBL "unreachable" False} -> 'a
-assume val failwith: string -> 'a (* TODO: refine with a monadic type *)
-assume val raise: exn -> 'a (* TODO: refine with a monadic type *)
+assume val failwith: string -> 'a (* TODO: refine with the Exn monad *)
+assume val raise: exn -> 'a       (* TODO: refine with the Exn monad *)
 assume val pipe_right: 'a -> ('a -> 'b) -> 'b
 assume val pipe_left: ('a -> 'b) -> 'a -> 'b
 assume val ignore: 'a -> unit
 assume val exit: int -> 'a
 assume val try_with: (unit -> 'a) -> (exn -> 'a) -> 'a
-
-(* Unrefined specifications for these functions for typing ML code *)
-assume val op_ColonEquals: ref 'a -> 'a -> unit
-assume val op_Dereference: ref 'a -> 'a
 assume val op_AmpAmp             : bool -> bool -> PURE.Tot bool
 assume val op_BarBar             : bool -> bool -> PURE.Tot bool
 assume val op_Negation           : bool -> PURE.Tot bool
